[[3-SAT]]

![[Pasted image 20241120154705.png]]


### put together

$$(\lnot A \lor X_{3}) \land (B \lor X_{3}) \land (\lnot X_{3} \lor A \lor \lnot B)$$
$$\land (\lnot X_{2} \lor \lnot X_{3} \lor C) \land (X_{2} \lor X_{3}) \land (X_{2} \lor \lnot C)$$
$$\land (\lnot X_{1} \lor A \lor C) \land (\lnot X_{1} \lor \lnot A \lor \lnot C) \land (X_{1} \lor \lnot A \lor C) \land (X_{1} \lor A \lor \lnot C)$$
$$ \land (\lnot X_{0} \lor \lnot X_{1})\land (\lnot X_{0} \lor X_{2}) \land (X_{0} \lor X_{1} \lor \lnot X_{2})$$
$$\land X_{0}$$
